wip

src/tactic/hammer/monomorphization2.lean
@@ -6,6 +6,13 @@ super
 local attribute [inline] decidable.to_bool bool.decidable_eq
 option.decidable_exists_mem
 
+meta def tactic.log_exception {α} (tac : tactic α) : tactic α | s :=
+match tac s with
+| x@(result.exception (some msg) pos st) :=
+  (tactic.trace (msg ()) >> (λ _, x) : tactic α) st
+| x := x
+end
+
 open native
 open expr
 open tactic
@@ -45,42 +52,60 @@ meta def monom2_core {α} (cheads : list expr) :
     -- TODO
     pure []
   | _ := collect_successes (e::cheads) $ λ ch, do
-    trace (ch, e),
-    unify e ch,
-    trace "ok",
+    unify ch e,
     monom2_core es cont
   end
 
-meta def monom2 (cheads : list expr) (lem : polym_lem) : tactic (list hol_tm) := do
+meta def monom2 (cheads : list expr) (lem : (expr × polym_lem)) : tactic (list (expr × hol_tm)) := do
 retrieve_or_else [] $
-monom2_core cheads lem.cs $ do
-prop ← lem.prop.instantiate_mvars,
+monom2_core cheads lem.2.cs $ do
+prop ← lem.2.prop.instantiate_mvars,
+trace prop,
 guard $ ¬ prop.has_expr_meta_var,
-pure [prop]
+pure [(lem.1, prop)]
 
-meta def monomorphization2_round (lems : list polym_lem) : tactic (list hol_tm) := do
-let cs := (do l ← lems, c ← l.prop.exprs, guard $ ¬ c.has_meta_var, pure c).dup_native,
-trace cs,
+meta def monomorphization2_round (lems : list (expr × polym_lem)) : tactic (list (expr × hol_tm)) := do
+let cs := (do (n,l) ← lems, c ← l.prop.exprs, guard $ ¬ c.has_meta_var, pure c).dup_native,
 lems' ← list.join <$> lems.mmap (monom2 cs),
-lems' ← lems'.mmap (λ lem, do t ← lem.to_expr, pure (t, lem)),
+lems' ← lems'.mmap (λ ⟨n, lem⟩, do t ← lem.to_expr, pure (t, n, lem)),
 let lems' := (lems'.group_by_native prod.fst).to_list.map (λ ⟨k, vs⟩, vs.head.2),
--- trace lems',
--- lems'.mmap infer_type >>= trace,
 pure lems'
 
-meta def monomorphize2 (lems : list expr) (rounds := 2) : tactic (list hol_tm) := do
-lems ← lems.mmap polym_lem.of_lemma,
-lems.mmap' (λ ⟨a,b⟩, trace(a,b)),
+meta def monomorphize2 (lems : list expr) (rounds := 2) : tactic (list (expr × hol_tm)) := do
+lems ← lems.mmap (λ n, prod.mk n <$> (infer_type n >>= polym_lem.of_lemma)),
 rounds.iterate (λ lems', do lems' ← lems',
-  monomorphization2_round (lems ++ lems'.map polym_lem.of_hol_tm)) (pure [])
+    monomorphization2_round (lems ++
+      lems'.map (λ ⟨n,l⟩, prod.mk n (polym_lem.of_hol_tm l))))
+  (pure [])
 
-meta def to_tf0.sort_name (e : expr) : to_tf0 string :=
-to_tf0.name_core e (λ n, "t" ++ tptpify_name n)
+meta def to_tf0.name'_core (e : expr) (f : name → string) : to_tf0 string := do
+ns ← to_tf0_state.ns <$> state_t.get,
+match ns.find e with
+| some n := pure n
+| none := do
+  state_t.modify $ λ st, { fresh_idx := st.fresh_idx + 1, ..st },
+  idx ← to_tf0_state.fresh_idx <$> state_t.get,
+  let n := f (name.mk_numeral (unsigned.of_nat idx) (hint_name e)),
+  state_t.modify $ λ st, { ns := st.ns.insert e n, ..st },
+  pure n
+end
+
+meta def to_tf0.var_name' (e : expr) : to_tf0 string :=
+to_tf0.name'_core e var_tptpify_name
+
+meta def to_tf0.con_name' (e : expr) : to_tf0 string :=
+to_tf0.name'_core e fn_tptpify_name
+
+meta def to_tf0.ax_name' (e : expr) : to_tf0 string :=
+to_tf0.name'_core e ax_tptpify_name
+
+meta def to_tf0.sort_name' (e : expr) : to_tf0 string :=
+to_tf0.name'_core e (λ n, "t" ++ tptpify_name n)
 
 meta mutual def to_tf0_hol_ty, to_tf0_hol_ty_fun
 with to_tf0_hol_ty : hol_ty → to_tf0 format
 | hol_ty.tbool := pure "$o"
-| (hol_ty.base t) := format.of_string <$> to_tf0.sort_name t
+| (hol_ty.base t) := format.of_string <$> to_tf0.sort_name' t
 | e@(hol_ty.arr _ _) := format.paren' <$> to_tf0_hol_ty_fun e
 with to_tf0_hol_ty_fun : hol_ty → to_tf0 format
 | (hol_ty.arr a b) := do
@@ -92,40 +117,36 @@ with to_tf0_hol_ty_fun : hol_ty → to_tf0 format
 @[pattern] meta def bin_lc (lc : hol_lcon) (a b : hol_tm) : hol_tm :=
 hol_tm.app (hol_tm.app (hol_tm.lcon lc) a) b
 
-meta def to_tf0_legalize : hol_tm → tactic hol_tm
-| e@(hol_tm.lcon hol_lcon.true) := pure e
-| e@(hol_tm.lcon hol_lcon.false) := pure e
-| e@(hol_tm.var i) := pure e
-| e@(hol_tm.con n _) := pure e
-| (bin_lc (hol_lcon.eq t) x y) := bin_lc (hol_lcon.eq t) <$> to_tf0_legalize x <*> to_tf0_legalize y
-| (bin_lc hol_lcon.and x y) := bin_lc hol_lcon.and <$> to_tf0_legalize x <*> to_tf0_legalize y
-| (bin_lc hol_lcon.or x y) := bin_lc hol_lcon.or <$> to_tf0_legalize x <*> to_tf0_legalize y
-| (bin_lc hol_lcon.iff x y) := bin_lc hol_lcon.iff <$> to_tf0_legalize x <*> to_tf0_legalize y
-| (bin_lc hol_lcon.imp x y) := bin_lc hol_lcon.imp <$> to_tf0_legalize x <*> to_tf0_legalize y
-| (hol_tm.app (hol_tm.lcon hol_lcon.neg) x) := hol_tm.app (hol_tm.lcon hol_lcon.neg) <$> to_tf0_legalize x
-| (hol_tm.app (hol_tm.lcon $ hol_lcon.ex t0) (hol_tm.lam x t a)) :=
-  (hol_tm.app (hol_tm.lcon $ hol_lcon.ex t0) ∘ hol_tm.lam x t) <$> to_tf0_legalize a
-| (hol_tm.app (hol_tm.lcon $ hol_lcon.all t0) (hol_tm.lam x t a)) :=
-  (hol_tm.app (hol_tm.lcon $ hol_lcon.all t0) ∘ hol_tm.lam x t) <$> to_tf0_legalize a
-| (hol_tm.app a b) := hol_tm.app <$> to_tf0_legalize a <*> to_tf0_legalize b
-| (hol_tm.lam x t a) := hol_tm.lam x t <$> to_tf0_legalize a
-| (hol_tm.cast t a) := do
-  def_eq ← option.is_some <$> try_core (is_def_eq a.ty.to_expr t.to_expr),
-  n ← to_expr $
-    if def_eq then
-      ``(cast rfl : %%a.ty.to_expr → %%t.to_expr)
-    else
-      ``(cast sorry : %%a.ty.to_expr → %%t.to_expr),
-  to_tf0_legalize (hol_tm.app (hol_tm.con n (a.ty.arr t)) a)
-| (hol_tm.lcon lc) := do e ← lc.to_expr, to_tf0_legalize $ hol_tm.con e lc.ty
+meta def to_tf0_legalize : hol_tm → list hol_ty → tactic hol_tm
+| e@(hol_tm.lcon hol_lcon.true) lctx := pure e
+| e@(hol_tm.lcon hol_lcon.false) lctx := pure e
+| e@(hol_tm.var i) lctx := pure e
+| e@(hol_tm.con n _) lctx := pure e
+| (bin_lc (hol_lcon.eq t) x y) lctx := bin_lc (hol_lcon.eq t) <$> to_tf0_legalize x lctx <*> to_tf0_legalize y lctx
+| (bin_lc hol_lcon.and x y) lctx := bin_lc hol_lcon.and <$> to_tf0_legalize x lctx <*> to_tf0_legalize y lctx
+| (bin_lc hol_lcon.or x y) lctx := bin_lc hol_lcon.or <$> to_tf0_legalize x lctx <*> to_tf0_legalize y lctx
+| (bin_lc hol_lcon.iff x y) lctx := bin_lc hol_lcon.iff <$> to_tf0_legalize x lctx <*> to_tf0_legalize y lctx
+| (bin_lc hol_lcon.imp x y) lctx := bin_lc hol_lcon.imp <$> to_tf0_legalize x lctx <*> to_tf0_legalize y lctx
+| (hol_tm.app (hol_tm.lcon hol_lcon.neg) x) lctx := hol_tm.app (hol_tm.lcon hol_lcon.neg) <$> to_tf0_legalize x lctx
+| (hol_tm.app (hol_tm.lcon $ hol_lcon.ex t0) (hol_tm.lam x t a)) lctx :=
+  (hol_tm.app (hol_tm.lcon $ hol_lcon.ex t0) ∘ hol_tm.lam x t) <$> to_tf0_legalize a (t :: lctx)
+| (hol_tm.app (hol_tm.lcon $ hol_lcon.all t0) (hol_tm.lam x t a)) lctx :=
+  (hol_tm.app (hol_tm.lcon $ hol_lcon.all t0) ∘ hol_tm.lam x t) <$> to_tf0_legalize a (t :: lctx)
+| (hol_tm.app a b) lctx := hol_tm.app <$> to_tf0_legalize a lctx <*> to_tf0_legalize b lctx
+| (hol_tm.lam x t a) lctx := hol_tm.lam x t <$> to_tf0_legalize a (t :: lctx)
+| (hol_tm.cast t a) lctx := do
+  let ta := a.ty_core lctx,
+  n ← to_expr ``(cast sorry : %%ta.to_expr → %%t.to_expr),
+  to_tf0_legalize (hol_tm.app (hol_tm.con n (ta.arr t)) a) lctx
+| (hol_tm.lcon lc) lctx := do e ← lc.to_expr, to_tf0_legalize (hol_tm.con e lc.ty) lctx
 
 meta def to_tf0_hol_tm : list (name × hol_ty) → hol_tm → to_tf0 format
 | lctx (hol_tm.lcon hol_lcon.true) := pure "$true"
 | lctx (hol_tm.lcon hol_lcon.false) := pure "$false"
 | lctx (hol_tm.var i) :=
   let ⟨n, t⟩ := lctx.inth i in
-  format.of_string <$> to_tf0.var_name (expr.local_const n n binder_info.default t.to_expr)
-| lctx (hol_tm.con n _) := format.of_string <$> to_tf0.con_name n
+  format.of_string <$> to_tf0.var_name' (expr.local_const n n binder_info.default t.to_expr)
+| lctx (hol_tm.con n _) := format.of_string <$> to_tf0.con_name' n
 | lctx (hol_tm.app (hol_tm.app (hol_tm.lcon $ hol_lcon.eq _) x) y) :=
   tptpify_binop "=" <$> to_tf0_hol_tm lctx x <*> to_tf0_hol_tm lctx y
 | lctx (hol_tm.app (hol_tm.app (hol_tm.lcon $ hol_lcon.and) x) y) :=
@@ -141,11 +162,11 @@ meta def to_tf0_hol_tm : list (name × hol_ty) → hol_tm → to_tf0 format
   pure $ format.paren' $ "~" ++ format.line ++ x'
 | lctx (hol_tm.app (hol_tm.lcon $ hol_lcon.ex _) (hol_tm.lam x t a)) := do
   let x' := x.mk_numeral lctx.length,
-  tptpify_quant' "?" <$> to_tf0.var_name (expr.local_const x' x' binder_info.default t.to_expr) <*>
+  tptpify_quant' "?" <$> to_tf0.var_name' (expr.local_const x' x' binder_info.default t.to_expr) <*>
     to_tf0_hol_ty t <*> to_tf0_hol_tm ((x', t) :: lctx) a
 | lctx (hol_tm.app (hol_tm.lcon $ hol_lcon.all _) (hol_tm.lam x t a)) := do
   let x' := x.mk_numeral lctx.length,
-  tptpify_quant' "!" <$> to_tf0.var_name (expr.local_const x' x' binder_info.default t.to_expr) <*>
+  tptpify_quant' "!" <$> to_tf0.var_name' (expr.local_const x' x' binder_info.default t.to_expr) <*>
     to_tf0_hol_ty t <*> to_tf0_hol_tm ((x', t) :: lctx) a
 | lctx e@(hol_tm.app _ _) :=
   let fn := e.get_app_fn, as := e.get_app_args in
@@ -153,80 +174,79 @@ meta def to_tf0_hol_tm : list (name × hol_ty) → hol_tm → to_tf0 format
     <$> (fn :: as).mmap (to_tf0_hol_tm lctx)
 | lctx (hol_tm.lam x t a) := do
   let x' := x.mk_numeral lctx.length,
-  tptpify_quant' "^" <$> to_tf0.var_name (expr.local_const x' x' binder_info.default t.to_expr) <*>
+  tptpify_quant' "^" <$> to_tf0.var_name' (expr.local_const x' x' binder_info.default t.to_expr) <*>
     to_tf0_hol_ty t <*> to_tf0_hol_tm ((x', t) :: lctx) a
 | lctx e := state_t.lift $ do e ← pp e, fail $ to_fmt "to_tf0_hol_tm: unsupported: " ++ e
 
-meta def to_tf0_file2 (lems : list hol_tm) : to_tf0 (format × list (string × hol_tm)) := do
-lems ← state_t.lift $ lems.mmap to_tf0_legalize,
-let sorts := (lems.map hol_tm.sorts).join.dup_native,
+meta def to_tf0_file2 (lems : list (expr × hol_tm)) : to_tf0 (format × list (string × expr × hol_tm)) := do
+lems ← state_t.lift $ lems.mmap $ λ ⟨n, l⟩, prod.mk n <$> to_tf0_legalize l [],
+let sorts := (lems.map (hol_tm.sorts ∘ prod.snd)).join.dup_native,
 sort_decls ← sorts.mmap (λ c, do
-  c' ← to_tf0.sort_name c,
+  c' ← to_tf0.sort_name' c,
   pure $ tptpify_thf_ann "type" ("ty_" ++ c')
     (tptpify_binop ":" c' "$tType")),
--- state_t.lift $ trace (cs, lems),
-let cs := (lems.map hol_tm.consts).join.dup_native,
+let cs := (lems.map (hol_tm.consts ∘ prod.snd)).join.dup_native,
 ty_decls ← cs.mmap (λ ⟨c, t⟩, do
   t' ← to_tf0_hol_ty t,
-  c' ← to_tf0.con_name c,
+  c' ← to_tf0.con_name' c,
   pure $ tptpify_thf_ann "type" ("ty_" ++ c') (tptpify_binop ":" c' t')),
--- state_t.lift $ trace lems,
-axs ← lems.zip_with_index.mmap (λ ⟨ax, i⟩, do
-  let n := "ax" ++ to_string i,
+axs ← lems.mmap (λ ⟨pr, ax⟩, do
+  n ← to_tf0.ax_name' pr,
   ann ← tptpify_thf_ann "axiom" n <$> to_tf0_hol_tm [] ax,
-  pure (n, ax, ann)),
+  pure (n, pr, ax, ann)),
 let tptp := format.join $
-  ((sort_decls ++ ty_decls ++ axs.map (λ ⟨n,ax,ann⟩, ann)).map format.group)
+  ((sort_decls ++ ty_decls ++ axs.map (λ ⟨n,pr,ax,ann⟩, ann)).map format.group)
   .intersperse (format.line ++ format.line),
-pure (tptp, axs.map (λ ⟨n,ax,ann⟩, (n, ax)))
+pure (tptp, axs.map (λ ⟨n,pr,ax,ann⟩, (n, pr, ax)))
 
-meta def mk_monom2_file (axs : list name) : tactic (format × list (string × hol_tm)) := do
+meta def simplify_lems (lems : list (expr × hol_tm)) : tactic (list (expr × hol_tm)) :=
+prod.fst <$> state_t.run (lems.mmap (λ ⟨n, l⟩, prod.mk n <$> l.simplify [])) {}
+
+meta def mk_monom2_file (axs : list name) : tactic (format × list (string × expr × hol_tm)) := do
 goal ← retrieve (revert_all >> target),
 let axs := goal.constants.filter is_good_const ++ axs,
 axs ← close_under_references axs,
--- trace $ (axs.map name.to_string).qsort (λ a b, a < b),
 repeat (intro1 >> skip),
 (do tgt ← target, when (tgt ≠ `(false)) $
   mk_mapp ``classical.by_contradiction [some tgt] >>= eapply >> intro1 >> skip),
 lems ← (++) <$> axs.mmap mk_const <*> local_context,
 lems' ← monomorphize2 lems 2,
--- (cs'', lems'') ← intern_lems lems',
-let lems'' := lems',
+lems'' ← simplify_lems lems',
 (to_tf0_file2 lems'').run
 
--- meta def filter_lemmas2_core (tptp : format) (ax_names : list (string × expr × expr)) :
---   tactic (list (expr × expr)) := do
--- -- trace tptp,
--- (tactic.unsafe_run_io $ do f ← io.mk_file_handle "hammer.p" io.mode.write, io.fs.write f tptp.to_string.to_char_buffer, io.fs.close f),
--- let ax_names := rb_map.of_list ax_names,
--- -- (failure : tactic unit),
--- tptp_out ← timetac "eprover-ho took" $ exec_cmd "bash" ["-c",
---   "set -o pipefail; eprover-ho --cpu-limit=30 --proof-object=1 | " ++
---     "grep -oP '(?<=file\\(..stdin.., ).*?(?=\\))'"]
---   tptp.to_string,
--- let ns := tptp_out.split_on '\n',
--- pure $ do n ← ns, (ax_names.find n).to_list
+meta def filter_lemmas3_core (tptp : format) (ax_names : list (string × expr × hol_tm)) :
+  tactic (list (expr × hol_tm)) := do
+trace tptp,
+(tactic.unsafe_run_io $ do f ← io.mk_file_handle "hammer.p" io.mode.write, io.fs.write f tptp.to_string.to_char_buffer, io.fs.close f),
+let ax_names := rb_map.of_list ax_names,
+-- (failure : tactic unit),
+tptp_out ← timetac "eprover-ho took" $ exec_cmd "bash" ["-c",
+  "set -o pipefail; eprover-ho --cpu-limit=30 --proof-object=1 | " ++
+    "grep -oP '(?<=file\\(..stdin.., ).*?(?=\\))'"]
+  tptp.to_string,
+let ns := tptp_out.split_on '\n',
+pure $ do n ← ns, (ax_names.find n).to_list
 
--- meta def filter_lemmas2 (axs : list name) : tactic (list (expr × expr)) := do
--- (tptp, ax_names) ← mk_monom_file axs,
--- filter_lemmas2_core tptp ax_names
+meta def filter_lemmas3 (axs : list name) : tactic (list (expr × hol_tm)) := do
+(tptp, ax_names) ← mk_monom2_file axs,
+filter_lemmas3_core tptp ax_names
 
--- meta def find_lemmas2 (max := 10) : tactic (list (expr × expr)) := do
--- axs ← timetac "Premise selection took" $ retrieve $
---   revert_all >> target >>= select_for_goal,
--- let axs := (axs.take max).map (λ a, a.1),
--- -- trace "Premise selection:",
--- trace axs,
--- filter_lemmas2 axs
+meta def find_lemmas3 (max := 10) : tactic (list (expr × hol_tm)) := do
+axs ← timetac "Premise selection took" $ retrieve $
+  revert_all >> target >>= select_for_goal,
+let axs := (axs.take max).map (λ a, a.1),
+-- trace "Premise selection:",
+trace axs,
+filter_lemmas3 axs
 
--- meta def reconstruct2 (axs : list (expr × expr)) : tactic unit :=
--- focus1 $ super.with_ground_mvars $ do
--- axs ← axs.mmap $ λ ⟨pr, ty⟩, super.clause.of_type_and_proof ty pr,
--- super.solve_with_goal {} axs
+meta def reconstruct3 (axs : list (expr × hol_tm)) : tactic unit :=
+focus1 $ super.with_ground_mvars $ do
+axs ← axs.mmap $ λ ⟨pr, _⟩, super.clause.of_proof pr,
+super.solve_with_goal {} axs
 
-set_option pp.all true
-set_option profiler true
-set_option trace.type_context.is_def_eq true
+-- set_option pp.all true
+-- set_option profiler true
+-- set_option trace.type_context.is_def_eq true
 -- set_option trace.type_context.is_def_eq_detail true
 
 example (x y : ℤ) (h : x ∣ y) (h2 : x ≤ y) (h3 : ¬ x + y < 0)
@@ -237,12 +257,9 @@ l2 ← mk_const ``le_antisymm,
 l3 ← mk_const ``exists_congr,
 l4 ← mk_const ``zero_sub,
 let ls : list expr := l1 :: l2 :: l3 :: l4 :: ls,
-ls ← ls.mmap infer_type,
 -- ls ← (λ x, [x]) <$> get_local `h3,
 ls' ← monomorphize2 ls 3,
--- ls'' ← intern_lems ls',
-let ls'' := ls',
-trace_state,
+ls'' ← simplify_lems ls',
 trace ls'',
 -- ls''.mmap' (λ l'', (to_tf0_tm [] l''.2).run >>= trace),
 (to_tf0_file2 ls'').run >>= trace,
@@ -257,43 +274,45 @@ namespace tactic
 namespace interactive
 open interactive interactive.types lean.parser
 
--- meta def find_lemmas2 (axs : parse $ optional $ list_of ident) (max_lemmas := 100) : tactic unit := do
--- lems ←
---   match axs with
---   | none := hammer.find_lemmas2 max_lemmas
---   | some axs := do
---     axs.mmap' (λ ax, get_decl ax),
---     timetac "eprover-ho took" $
---       hammer.filter_lemmas2 axs
---   end,
--- trace "eprover-ho proof uses the following lemmas:",
--- lems.mmap' (λ ⟨l, t⟩, do
---   l' ← pp l,
---   -- t ← infer_type l >>= pp,
---   t ← pp t,
---   trace (format.nest 4 $ format.group $ "  " ++ l' ++ " :" ++ format.line ++ t)),
--- admit
+meta def find_lemmas3 (axs : parse $ optional $ list_of ident) (max_lemmas := 100) : tactic unit := do
+lems ←
+  match axs with
+  | none := hammer.find_lemmas3 max_lemmas
+  | some axs := do
+    axs.mmap' (λ ax, get_decl ax),
+    timetac "eprover-ho took" $
+      hammer.filter_lemmas3 axs
+  end,
+trace "eprover-ho proof uses the following lemmas:",
+lems.mmap' (λ ⟨l, t⟩, do
+  l' ← pp l,
+  -- t ← infer_type l >>= pp,
+  t ← pp t,
+  trace (format.nest 4 $ format.group $ "  " ++ l' ++ " :" ++ format.line ++ t)),
+admit
 
--- meta def hammer2 (axs : parse $ optional $ list_of ident) (max_lemmas := 100) : tactic unit := do
--- lems ←
---   match axs with
---   | none := hammer.find_lemmas2 max_lemmas
---   | some axs := do
---     axs.mmap' (λ ax, get_decl ax),
---     timetac "eprover-ho took" $
---       hammer.filter_lemmas2 axs
---   end,
--- trace "eprover-ho proof uses the following lemmas:",
--- lems.mmap' (λ ⟨l, t⟩, do
---   l' ← pp l,
---   -- t ← infer_type l >>= pp,
---   t ← pp t,
---   trace (format.nest 4 $ format.group $ "  " ++ l' ++ " :" ++ format.line ++ t)),
--- hammer.reconstruct2 lems
+meta def hammer3 (axs : parse $ optional $ list_of ident) (max_lemmas := 100) : tactic unit := do
+lems ←
+  match axs with
+  | none := hammer.find_lemmas3 max_lemmas
+  | some axs := do
+    axs.mmap' (λ ax, get_decl ax),
+    timetac "eprover-ho took" $
+      hammer.filter_lemmas3 axs
+  end,
+trace "eprover-ho proof uses the following lemmas:",
+lems.mmap' (λ ⟨l, t⟩, do
+  l' ← pp l,
+  -- t ← infer_type l >>= pp,
+  t ← pp t,
+  trace (format.nest 4 $ format.group $ "  " ++ l' ++ " :" ++ format.line ++ t)),
+hammer.reconstruct3 lems
 
 end interactive
 end tactic
 
--- set_option trace.super true
--- example (x y : ℤ) : x + y = y + x :=
--- by hammer2 [add_comm]
+#print ""
+
+set_option trace.super true
+example (x y : ℤ) : x + y = y + x :=
+by hammer3 --[add_comm]
